BaseDef.v
@@ -14,15 +14,15 @@ Definition atom_eqb_spec (s1 s2 : atom): reflect (s1 = s2) (atom_eqb s1 s2) := S
 
 (** Locally Nameless Functions: *)
 
-(** This Stale class gathers all free variables in type context, values, terms,
-  etc. *)
-Class Stale {D} A := stale : A -> D.
-
 Definition fv_of_set (s: aset): atom := fresh_string_of_set "x" s.
 Lemma fv_of_set_fresh (s: aset) : (fv_of_set s) ∉ s.
 Proof.
   apply fresh_string_of_set_fresh.
 Qed.
+
+(** This Stale class gathers all free variables in type context, values, terms,
+  etc. *)
+Class Stale {D} A := stale : A -> D.
 
 #[global]
 Instance atom_stale : @Stale aset atom := singleton.
@@ -45,7 +45,7 @@ Notation "e '^^' s" := (open 0 s e) (at level 20).
 
 Class Close A := close : atom -> nat -> A -> A.
 
-Notation "'{' x '<~' k '}' e" := (close x k e) (at level 0, k constr).
+Notation "'{' x '<~' k '}' e" := (close k x e) (at level 0, k constr).
 
 Notation "x '\\' e" := (close x 0 e) (at level 20).
 
@@ -54,3 +54,5 @@ Class Lc A := lc : A -> Prop.
 Class Typing G E T := has_type : G -> E -> T -> Prop.
 
 Notation "Γ '⊢' e '⋮' T" := (has_type Γ e T) (at level 20, e constr, T constr, Γ constr).
+
+Hint Unfold open close subst stale : class_simpl.
