LocallyNameless/LangLc.v
@@ -1,0 +1,1296 @@
+From stdpp Require Import mapset.
+From CT Require Import Syntax.Syntax.
+From CT Require Import MyTactics.
+Import Primitives.
+Import BaseDef.
+From Hammer Require Import Tactics.
+
+(** This file provides the infrastructure for reasoning about locally nameless
+  representation for the core language. Most lemmas in this file are inspired by
+  Arthur Chargu´eraud's paper "The Locally Nameless Representation" :
+  https://chargueraud.org/research/2009/ln/main.pdf *)
+
+Lemma constant_eqb_spec: forall (c c': constant), c = c' \/ c <> c'.
+Proof with eauto.
+  destruct c, c'...
+  - destruct b, b0; firstorder.
+  - destruct (Nat.eq_dec n n0); firstorder.
+    right. intro HH. inversion HH...
+Qed.
+
+Ltac specialize_L :=
+  match goal with
+  | [ H : forall (x: atom), x ∉ ?L -> _ |- _] => specialize (H (fv_of_set L) (fv_of_set_fresh L))
+  end.
+
+Lemma lc_exfalso: forall bn, ~ lc (vbvar bn).
+Proof.
+  intros bn HF. inversion HF.
+Qed.
+
+Lemma body_exfalso1: forall bn, ~ body (vbvar (S bn)).
+Proof.
+  intros bn HF. inversion HF. specialize_L. inversion H.
+Qed.
+
+Lemma body_exfalso: forall bn, ~ body (treturn (vbvar (S bn))).
+Proof.
+  intros bn HF. inversion HF. specialize_L. inversion H. inversion H1.
+Qed.
+
+Ltac solve_lc_exfalso :=
+  match goal with
+    | [ H: lc (treturn (vbvar ?n)) |- _ ] => exfalso; apply (lc_exfalso n); auto
+    | [ H: body (treturn (vbvar (S ?n))) |- _ ] => exfalso; apply (body_exfalso n); auto
+  end.
+
+Lemma lc_abs_iff_body: forall T e, lc (vlam T e) <-> body e.
+Proof.
+  split; unfold body; intros.
+  - inversion H; subst. exists L. auto.
+  - destruct H as (L & HL). eapply lc_vlam. apply HL.
+Qed.
+
+Lemma lc_return_iff_lc_value: forall v, lc (treturn v) <-> lc v.
+Proof.
+  split; intros.
+  - inversion H; subst. auto.
+  - constructor. auto.
+Qed.
+
+Ltac rewrite_by_set_solver :=
+  repeat
+  match goal with
+  | H: context [ _ ->  _ = _ ]  |- _ => erewrite H; eauto; fast_set_solver!!
+  end; auto.
+
+(* Ltac dec_tf := try (subst; rewrite decide_True; auto; fast_set_solver); try (rewrite decide_False; auto; fast_set_solver). *)
+
+(* We keep [Stale], [Open] and [Close] as explicit class parameters so that
+   the definition is well-typed for arbitrary [A], but in all our concrete
+   uses (e.g. [A = tm]) these parameters are instantiated with the canonical
+   global instances from [Syntax.Lang]. *)
+Class CloseOpenVar A `{Stale aset A} `{Open value A} `{Close A} := close_open_var :
+  forall (e: A) (x: atom) (k: nat), x # e -> {k <~ x} ({k ~> (vfvar x)} e) = e.
+
+#[global] Instance CloseOpenVar_tm : CloseOpenVar tm.
+Proof.
+  unfold CloseOpenVar.
+  apply (tm_mutual_rec
+           (fun (v: value) => forall (x: atom) (k: nat), x # v -> {k <~ x} ({k ~> (vfvar x)} v) = v)
+           (fun (e: tm) => forall (x: atom) (k: nat), x # e -> {k <~ x} ({k ~> (vfvar x)} e) = e)
+        ); autounfold with class_simpl; simpl; intros; mydestr; try f_equal; rewrite_by_set_solver.
+  - my_set_solver.
+  - hauto.
+Qed.
+Arguments CloseOpenVar_tm /.
+
+#[global] Instance CloseOpenVar_value : CloseOpenVar value.
+Proof.
+  unfold CloseOpenVar.
+  apply (value_mutual_rec
+           (fun (v: value) => forall (x: atom) (k: nat), x # v -> {k <~ x} ({k ~> (vfvar x)} v) = v)
+           (fun (e: tm) => forall (x: atom) (k: nat), x # e -> {k <~ x} ({k ~> (vfvar x)} e) = e)
+        ); autounfold with class_simpl; simpl; intros; mydestr; try f_equal; rewrite_by_set_solver.
+  - my_set_solver.
+  - hauto.
+Qed.
+Arguments CloseOpenVar_value /.
+
+Class OpenFv A `{Stale aset A} `{Open value A} := open_fv :
+   forall (v: A) (u: value) (k: nat), 
+   stale ({k ~> u} v) ⊆ stale u ∪ stale v.
+
+#[global] Instance OpenFv_value : OpenFv value.
+Proof.
+  unfold OpenFv.
+  apply (value_mutual_rec
+           (fun (v: value) => forall (u: value) (k: nat), fv_value ({k ~> u} v) ⊆ fv_value u ∪ fv_value v)
+           (fun (e: tm) => forall (u: value) (k: nat), fv_tm ({k ~> u} e) ⊆ fv_value u ∪ fv_tm e)
+        ); autounfold with class_simpl; simpl; intros; mydestr;
+    try (intros; repeat rewrite_by_set_solver; auto);
+    set_solver.
+Qed.
+Arguments OpenFv_value /.
+
+#[global] Instance OpenFv_tm : OpenFv tm.
+Proof.
+  unfold OpenFv.
+  apply (tm_mutual_rec
+           (fun (v: value) => forall (u: value) (k: nat), stale ({k ~> u} v) ⊆ stale u ∪ stale v)
+           (fun (e: tm) => forall (u: value) (k: nat), stale ({k ~> u} e) ⊆ stale u ∪ stale e)
+        ); autounfold with class_simpl; simpl; intros; mydestr;
+    try (intros; repeat rewrite_by_set_solver; auto); set_solver.
+Qed.
+Arguments OpenFv_tm /.
+
+Class OpenFvPrime A `{Stale aset A} `{Open value A} := open_fv' :
+forall (v: A) (u: value) (k: nat), stale v ⊆ stale ({k ~> u} v).
+
+#[global] Instance OpenFvPrime_value : OpenFvPrime value.
+Proof.
+  unfold OpenFvPrime.
+  apply (value_mutual_rec
+           (fun (v: value) => forall (u: value) (k: nat), stale v ⊆ stale ({k ~> u} v))
+           (fun (e: tm) => forall (u: value) (k: nat), stale e ⊆ stale ({k ~> u} e))
+        ); autounfold with class_simpl; simpl; intros; mydestr;
+    try (intros; repeat rewrite_by_set_solver; auto); set_solver.
+Qed.
+Arguments OpenFvPrime_value /.
+
+#[global] Instance OpenFvPrime_tm : OpenFvPrime tm.
+Proof.
+  unfold OpenFvPrime.
+  apply (tm_mutual_rec
+           (fun (v: value) => forall (u: value) (k: nat), stale v ⊆ stale ({k ~> u} v))
+           (fun (e: tm) => forall (u: value) (k: nat), stale e ⊆ stale ({k ~> u} e))
+        ); autounfold with class_simpl; simpl; intros; mydestr;
+    try (intros; repeat rewrite_by_set_solver; auto); set_solver.
+Qed.
+Arguments OpenFvPrime_tm /.
+
+Class CloseVarFv A `{Stale aset A} `{Close A} := close_var_fv :
+forall (v: A) (x: atom) (k: nat), stale ({k <~ x} v) = (stale v) ∖ {[x]}.
+
+#[global] Instance CloseVarFv_value : CloseVarFv value.
+Proof.
+  unfold CloseVarFv.
+  apply (value_mutual_rec
+           (fun (v: value) => forall (x: atom) (k: nat), stale ({k <~ x} v) = (stale v) ∖ {[x]})
+           (fun (e: tm) => forall (x: atom) (k: nat), stale ({k <~ x} e) = (stale e) ∖ {[x]})
+        ); autounfold with class_simpl; simpl; intros; mydestr; rewrite_by_set_solver.
+        all: my_set_solver.
+Qed.
+Arguments CloseVarFv_value /.
+
+#[global] Instance CloseVarFv_tm : CloseVarFv tm.
+Proof.
+  unfold CloseVarFv.
+  apply (tm_mutual_rec
+           (fun (v: value) => forall (x: atom) (k: nat), stale ({k <~ x} v) = (stale v) ∖ {[x]})
+           (fun (e: tm) => forall (x: atom) (k: nat), stale ({k <~ x} e) = (stale e) ∖ {[x]})
+        ); autounfold with class_simpl; simpl; intros; mydestr; rewrite_by_set_solver.
+        all: my_set_solver.
+Qed.
+Arguments CloseVarFv_tm /.
+
+Class SubstFresh A `{Stale aset A} `{Subst value A} := subst_fresh :
+forall (v: A) (x:atom) (u: value), x # v -> {x := u} v = v.
+
+#[global] Instance SubstFresh_value : SubstFresh value.
+Proof.
+  unfold SubstFresh.
+  apply (value_mutual_rec
+           (fun (v: value) => forall (x:atom) (u: value), x # v -> {x := u} v = v)
+           (fun (e: tm) => forall (x:atom) (u: value), x # e -> {x := u} e = e)
+        ); autounfold with class_simpl; simpl; intros; mydestr; try f_equal; rewrite_by_set_solver.
+        - my_set_solver.
+Qed.
+Arguments SubstFresh_value /.
+
+#[global] Instance SubstFresh_tm : SubstFresh tm.
+Proof.
+  unfold SubstFresh.
+  apply (tm_mutual_rec
+           (fun (v: value) => forall (x:atom) (u: value), x ∉ (fv_value v) -> {x := u} v = v)
+           (fun (e: tm) => forall (x:atom) (u: value), x ∉ (fv_tm e) -> {x := u} e = e)
+        ); autounfold with class_simpl; simpl; intros; mydestr; try f_equal; rewrite_by_set_solver.
+        - my_set_solver.
+Qed.
+Arguments SubstFresh_tm /.
+
+Ltac ex_specialize_L :=
+  match goal with
+  | [ H : ex (fun (L: aset) => _) |- _] => destruct H; specialize_L
+  end.
+
+(** There is a typo in the paper *)
+Class Fact1 A `{Stale aset A} `{Open value A} := fact1 :
+forall (u v: value) (e: A) i j,
+    i <> j -> {i ~> u} ({j ~> v} e) = {j ~> v} e -> {i ~> u} e = e.
+
+#[global] Instance Fact1_tm : Fact1 tm.
+Proof.
+  unfold Fact1.
+  intros u v.
+  apply (tm_mutual_rec
+  (fun (e: value) => forall i j, i <> j -> {i ~> u} ({j ~> v} e) = {j ~> v} e -> {i ~> u} e = e)
+  (fun (e: tm) => forall i j, i <> j -> {i ~> u} ({j ~> v} e) = {j ~> v} e -> {i ~> u} e = e)
+); autounfold with class_simpl; simpl; intros; mydestr; rewrite_by_set_solver; try hauto.
+Qed.
+Arguments Fact1_tm /.
+
+#[global] Instance Fact1_value : Fact1 value.
+Proof.
+  unfold Fact1.
+  intros u v.
+  apply (value_mutual_rec
+           (fun (e: value) => forall i j, i <> j -> {i ~> u} ({j ~> v} e) = {j ~> v} e -> {i ~> u} e = e)
+           (fun (e: tm) => forall i j, i <> j -> {i ~> u} ({j ~> v} e) = {j ~> v} e -> {i ~> u} e = e)
+        ); autounfold with class_simpl; simpl; intros; mydestr; rewrite_by_set_solver; try hauto.
+Qed.
+Arguments Fact1_value /.
+
+Ltac solve_let_lc_body H :=
+  split; intros; try repeat split; auto;
+    inversion H; subst; auto;
+    try destruct_hyp_conj; try match goal with
+    | [ H: body _ |- _ ] => inversion H; subst; clear H
+    (* | [ H: lc _ |- _ ] => inversion H; subst; clear H *)
+    end;
+    auto_exists_L; intros; repeat split; auto;
+    auto_apply; my_set_solver.
+
+Lemma lete_lc_body: forall e1 e, lc (tlete e1 e) <-> lc e1 /\ body e.
+Proof.
+  solve_let_lc_body H.
+Qed.
+
+Lemma letapp_lc_body: forall (v1 v2: value) e, lc (tletapp v1 v2 e) <-> lc v1 /\ lc v2 /\ body e.
+Proof.
+  solve_let_lc_body H.
+Qed.
+
+Lemma leteffop_lc_body: forall op (v1: value) e, lc (tleteffop op v1 e) <-> lc v1 /\ body e.
+Proof.
+  solve_let_lc_body H.
+Qed.
+
+Lemma match_lc_body: forall (v: value) e1 e2, lc (tmatchb v e1 e2) <-> lc v /\ lc e1 /\ lc e2.
+Proof.
+  solve_let_lc_body H.
+Qed.
+
+Lemma lc_fix_iff_body: forall T e, lc (vfix T e) <-> body e.
+Proof.
+  split; unfold body; intros.
+  - inversion H; subst. exists L. auto.
+  - destruct H as (L & HL). econstructor. apply HL.
+Qed.
+
+Ltac lc_solver_aux1:=
+  match goal with
+    | [H: lc (vbvar _) |- _ ] => inversion H
+    | [H: lc (treturn _) |- _ ] => rewrite lc_return_iff_lc_value in H; auto
+    | [H: lc (tlete _ _) |- body _ ] => rewrite lete_lc_body in H; mydestr; auto
+    | [H: lc (tletapp _ _ _) |- body _ ] => rewrite letapp_lc_body in H; mydestr; auto
+    | [H: lc (tleteffop _ _ _) |- body _ ] => rewrite leteffop_lc_body in H; mydestr; auto
+    | [H: lc (vlam _ _) |- body _ ] => rewrite lc_abs_iff_body in H; mydestr; auto
+    | [H: lc (vfix _ _) |- body _ ] => rewrite lc_fix_iff_body in H; mydestr; auto
+    | [H: lc (tlete _ _) |- lc _ ] => rewrite lete_lc_body in H; mydestr; auto
+    | [H: lc (tletapp _ _ _) |- lc _ ] => rewrite letapp_lc_body in H; mydestr; auto
+    | [H: lc (tleteffop _ _ _) |- lc _ ] => rewrite leteffop_lc_body in H; mydestr; auto
+    | [H: lc (tmatchb _ _ _) |- lc _ ] => rewrite match_lc_body in H; mydestr; auto
+    | [H: lc (vlam _ _) |- lc _ ] => rewrite lc_abs_iff_body in H; mydestr; auto
+    | [H: lc (vfix _ _) |- lc _ ] => rewrite lc_fix_iff_body in H; mydestr; auto
+    | [ |- lc (treturn _)] => apply lc_treturn; auto
+    | [ |- lc (terr _)] => apply lc_terr; auto
+    | [ |- lc (vconst _)] => apply lc_vconst; auto
+    | [ |- lc (vfvar _)] => constructor
+    | [ |- lc (tmatchb _ _ _)] => apply lc_tmatchb; (repeat split; auto)
+    | [ |- lc (tletapp _ _ _)] => rewrite letapp_lc_body; (repeat split; auto)
+    | [ |- lc (tleteffop _ _ _)] => rewrite leteffop_lc_body; (repeat split; auto)
+    | [ |- lc (tlete _ _)] => rewrite lete_lc_body; split; auto
+    | [ |- lc (vfix _ _)] => rewrite lc_fix_iff_body; auto
+    | [ |- lc (vlam _ _)] => rewrite lc_abs_iff_body; auto
+    | [ |- lc (treturn _)] => rewrite lc_return_iff_lc_value; auto
+    | [ |- lc (tmatchb _ _ _)] => rewrite match_lc_body; (repeat split; auto)
+    end.
+
+Ltac lc_solver1:= 
+  autounfold with class_simpl; simpl; mydestr; auto;
+  repeat (lc_solver_aux1; auto); fold_syntax_class.
+
+(* Lemma treturn_eq: forall (v1 v2: value), treturn v1 = treturn v2 -> v1 = v2.
+Proof.
+  intros. inversion H. auto.
+Qed. *)
+
+Class OpenRecLc A `{Stale aset A} `{Open value A} `{Lc A} := open_rec_lc :
+forall (e: A), lc e -> forall (k: nat) (v: value), {k ~> v} e = e.
+
+#[global] Instance OpenRecLc_tm : OpenRecLc tm.
+Proof.
+  unfold OpenRecLc.
+  apply (lc_tm_mutual_rec
+  (fun (e: value) _ => forall k (v: value), {k ~> v} e = e)
+  (fun (e: tm) _ => forall k (v: value), {k ~> v} e = e)
+  ); autounfold with class_simpl; simpl; intros; mydestr; f_equal; rewrite_by_set_solver; try hauto.   
+  all:
+    pose_fresh_fv y;
+    apply fact1 with (j := 0) (v:= y); auto; auto_apply; my_set_solver.
+Qed.
+Arguments OpenRecLc_tm /.
+
+#[global] Instance OpenRecLc_value : OpenRecLc value.
+Proof.
+  unfold OpenRecLc.
+  apply (lc_value_mutual_rec
+  (fun (e: value) _ => forall k (v: value), {k ~> v} e = e)
+  (fun (e: tm) _ => forall k (v: value), {k ~> v} e = e)
+  ); autounfold with class_simpl; simpl; intros; mydestr; f_equal; rewrite_by_set_solver; try hauto.   
+  all:
+    pose_fresh_fv y;
+    apply fact1 with (j := 0) (v:= y); auto; auto_apply; my_set_solver.
+Qed.
+Arguments OpenRecLc_value /.
+
+Class SubstOpen A `{Stale aset A} `{Open value A} `{Subst value A}  `{Lc A} := subst_open :
+forall (e: A) (u: value) (w: value) (x:atom) (k: nat),
+    lc w -> {x := w} ({k ~> u} e) = ({k ~> {x := w} u} ({x := w} e)).
+
+#[global] Instance SubstOpen_tm : SubstOpen tm.
+Proof.
+  unfold SubstOpen.
+  apply (tm_mutual_rec
+  (fun (e: value) => forall (u: value) (w: value) (x:atom) (k: nat), lc w -> {x := w} ({k ~> u} e) = ({k ~> {x := w} u} ({x := w} e)))
+  (fun (e: tm) => forall (u: value) (w: value) (x:atom) (k: nat), lc w -> {x := w} ({k ~> u} e) = ({k ~> {x := w} u} ({x := w} e)))
+); autounfold with class_simpl; simpl; intros; mydestr; try f_equal; auto.
+  - fold_syntax_class. repeat rewrite open_rec_lc; lc_solver1.
+Qed.
+Arguments SubstOpen_tm /.
+
+#[global] Instance SubstOpen_value : SubstOpen value.
+Proof.
+  unfold SubstOpen.
+  apply (value_mutual_rec
+           (fun (e: value) => forall (u: value) (w: value) (x:atom) (k: nat), lc w -> {x := w} ({k ~> u} e) = ({k ~> {x := w} u} ({x := w} e)))
+           (fun (e: tm) => forall (u: value) (w: value) (x:atom) (k: nat), lc w -> {x := w} ({k ~> u} e) = ({k ~> {x := w} u} ({x := w} e)))
+        ); autounfold with class_simpl; simpl; intros; mydestr; try f_equal; auto.
+  - fold_syntax_class. repeat rewrite open_rec_lc; lc_solver1.
+Qed.
+Arguments SubstOpen_value /.
+
+Class CloseVarRename A `{Stale aset A} `{Close A} `{Subst value A} := close_var_rename :
+forall (e: A) (x:atom) (y:atom) (k: nat),
+    y # e -> {k <~ x} e = {k <~ y} ({x := vfvar y} e).
+
+#[global] Instance CloseVarRename_tm : CloseVarRename tm.
+Proof.
+  unfold CloseVarRename.
+  apply (tm_mutual_rec
+           (fun (e: value) => forall (x:atom) (y:atom) (k: nat), y # e -> {k <~ x} e = {k <~ y} ({x := vfvar y} e))
+           (fun (e: tm) => forall (x:atom) (y:atom) (k: nat), y # e -> {k <~ x} e = {k <~ y} ({x := vfvar y} e))
+        ); autounfold with class_simpl; simpl; intros; mydestr; try f_equal; try (repeat rewrite_by_set_solver; auto).
+  - hauto.
+  - simpl; mydestr; auto. set_solver.
+Qed.
+Arguments CloseVarRename_tm /.
+
+#[global] Instance CloseVarRename_value : CloseVarRename value.
+Proof.
+  unfold CloseVarRename.
+  apply (value_mutual_rec
+           (fun (e: value) => forall (x:atom) (y:atom) (k: nat), y # e -> {k <~ x} e = {k <~ y} ({x := vfvar y} e))
+           (fun (e: tm) => forall (x:atom) (y:atom) (k: nat), y # e -> {k <~ x} e = {k <~ y} ({x := vfvar y} e))
+        ); autounfold with class_simpl; simpl; intros; mydestr; try f_equal; try (repeat rewrite_by_set_solver; auto).
+  - hauto.
+  - simpl; mydestr; auto. set_solver.
+Qed.
+Arguments CloseVarRename_value /.
+
+(* The second class of lemmas *)
+
+Ltac rewrite_by_set_solver2 :=
+  repeat match goal with
+          | H: context [ _ ->  _ = _ ]  |- _ => erewrite H by (eauto; my_set_solver)
+          end; auto.
+
+Class Fact2 A `{Stale aset A} `{Open value A} `{Close A} := fact2 :
+forall (e: A) (x y z: atom) (i j: nat),
+    x <> y -> i <> j -> y # e ->
+    {i ~> vfvar y} ({j ~> vfvar z} ({j <~ x} e)) = {j ~> vfvar z} ({j <~ x} ({i ~> vfvar y} e)).
+
+#[global] Instance Fact2_tm : Fact2 tm.
+Proof.
+  unfold Fact2.
+  apply (tm_mutual_rec
+           (fun (e: value) => forall (x:atom) (y:atom) (z:atom) (i j: nat), x <> y -> i <> j -> y # e -> {i ~> vfvar y} ({j ~> vfvar z} ({j <~ x} e)) = {j ~> vfvar z} ({j <~ x} ({i ~> vfvar y} e)))
+           (fun (e: tm) => forall (x:atom) (y:atom) (z:atom) (i j: nat), x <> y -> i <> j -> y # e -> {i ~> vfvar y} ({j ~> vfvar z} ({j <~ x} e)) = {j ~> vfvar z} ({j <~ x} ({i ~> vfvar y} e)))
+        ); autounfold with class_simpl; simpl; intros; mydestr; auto; 
+        rewrite_by_set_solver2.
+        all: simpl; mydestr; hauto.
+Qed.
+
+#[global] Instance Fact2_value : Fact2 value.
+Proof.
+  unfold Fact2.
+  apply (value_mutual_rec
+           (fun (e: value) => forall (x:atom) (y:atom) (z:atom) (i j: nat), x <> y -> i <> j -> y # e -> {i ~> vfvar y} ({j ~> vfvar z} ({j <~ x} e)) = {j ~> vfvar z} ({j <~ x} ({i ~> vfvar y} e)))
+           (fun (e: tm) => forall (x:atom) (y:atom) (z:atom) (i j: nat), x <> y -> i <> j -> y # e -> {i ~> vfvar y} ({j ~> vfvar z} ({j <~ x} e)) = {j ~> vfvar z} ({j <~ x} ({i ~> vfvar y} e)))
+        ); autounfold with class_simpl; simpl; intros; mydestr; auto; 
+        rewrite_by_set_solver2.
+        all: simpl; mydestr; hauto.
+Qed.
+Arguments Fact2_value /.
+
+Ltac ln_simpl :=
+autounfold with class_simpl in *; simpl in *; mydestr; do 3 fold_syntax_class.
+
+Class SubstLc A `{Stale aset A} `{Subst value A} `{Lc A} := subst_lc :
+forall (e: A), lc e -> forall (x:atom) (u: value), lc u -> lc ({x := u} e).
+
+#[global] Instance SubstLc_tm : SubstLc tm.
+Proof.
+  unfold SubstLc.
+  apply (lc_tm_mutual_rec
+           (fun (e: value) _ => forall (x:atom) (u: value), lc u -> lc ({x := u} e))
+           (fun (e: tm) _ => forall (x:atom) (u: value), lc u -> lc ({x := u} e))
+        ); ln_simpl; intros; auto;
+        try solve [lc_solver1; hauto].
+  all: auto_exists_L; intros; repeat split; fold_syntax_class; auto;
+    repeat match goal with
+      | [ H : forall z, z ∉ ?L -> _ |- lc (_ _ (vfvar ?y) _)] =>
+      assert (Hy : y ∉ L) by set_solver;
+      specialize (H y Hy)
+      | [ H : forall x u, _ -> lc _ , H1 : lc ?u |- context [ subst ?x ?u _ ]] =>
+      specialize (H x u H1);
+      rewrite subst_open in H; ln_simpl; set_solver
+    end.
+Qed.
+Arguments SubstLc_tm /.
+
+#[global] Instance SubstLc_value : SubstLc value.
+Proof.
+  unfold SubstLc.
+  apply (lc_value_mutual_rec
+           (fun (e: value) _ => forall (x:atom) (u: value), lc u -> lc ({x := u} e))
+           (fun (e: tm) _ => forall (x:atom) (u: value), lc u -> lc ({x := u} e))
+        ); ln_simpl; intros; auto;
+        try solve [lc_solver1; hauto].
+  all: auto_exists_L; intros; repeat split; fold_syntax_class; auto;
+    repeat match goal with
+      | [ H : forall z, z ∉ ?L -> _ |- lc (_ _ (vfvar ?y) _)] =>
+      assert (Hy : y ∉ L) by set_solver;
+      specialize (H y Hy)
+      | [ H : forall x u, _ -> lc _ , H1 : lc ?u |- context [ subst ?x ?u _ ]] =>
+      specialize (H x u H1);
+      rewrite subst_open in H; ln_simpl; set_solver
+    end.
+Qed.
+Arguments SubstLc_value /.
+
+Class OpenCloseVarAux A `{Stale aset A} `{Open value A} `{Close A} := open_close_var_aux :
+forall (e: A) (x: atom) (k: nat),
+    {k ~> (vfvar x)} e = e -> {k ~> (vfvar x)} ({k <~ x} e) = e.
+
+#[global] Instance OpenCloseVarAux_tm : OpenCloseVarAux tm.
+Proof.
+  unfold OpenCloseVarAux.
+  apply (tm_mutual_rec
+           (fun (e: value) => forall (x:atom) (k: nat), {k ~> (vfvar x)} e = e -> {k ~> (vfvar x)} ({k <~ x} e) = e)
+           (fun (e: tm) => forall (x:atom) (k: nat), {k ~> (vfvar x)} e = e -> {k ~> (vfvar x)} ({k <~ x} e) = e));
+    ln_simpl; intros; auto; f_equal_hyp;
+    try hauto.
+  - repeat ln_simpl; hauto.
+Qed.
+Arguments OpenCloseVarAux_tm /.
+
+#[global] Instance OpenCloseVarAux_value : OpenCloseVarAux value.
+Proof.
+  unfold OpenCloseVarAux.
+  apply (value_mutual_rec
+           (fun (e: value) => forall (x:atom) (k: nat), {k ~> (vfvar x)} e = e -> {k ~> (vfvar x)} ({k <~ x} e) = e)
+           (fun (e: tm) => forall (x:atom) (k: nat), {k ~> (vfvar x)} e = e -> {k ~> (vfvar x)} ({k <~ x} e) = e));
+    ln_simpl; intros; auto; f_equal_hyp;
+    try hauto.
+  - repeat ln_simpl; hauto.
+Qed.
+Arguments OpenCloseVarAux_value /.
+
+Class OpenCloseVar A `{Stale aset A} `{Open value A} `{Close A} `{Lc A} := open_close_var :
+forall (e: A) (x: atom), lc e -> {0 ~> (vfvar x)} ({0 <~ x} e) = e.
+
+#[global] Instance OpenCloseVar_all
+  (A : Type)
+  (staleA : Stale A)
+  (openA  : Open value A)
+  (closeA : Close A)
+  (lcA    : Lc A)
+  (openCloseVarAuxA : @OpenCloseVarAux A staleA openA closeA)
+  (openRecLcA       : @OpenRecLc       A staleA openA lcA)
+  : @OpenCloseVar A staleA openA closeA lcA.
+Proof.
+  unfold OpenCloseVar. intros e x Hlc.
+  apply open_close_var_aux.
+  apply open_rec_lc; auto.
+Qed.
+
+(* The third class of lemmas *)
+
+Class SubstIntro A `{Stale aset A} `{Open value A} `{Subst value A} `{Lc A} := subst_intro :
+forall (e: A) (x:atom) (w: value) (k: nat),
+    x # e ->
+    lc w -> {x := w} ({k ~> (vfvar x)} e) = ({k ~> w} e).
+
+#[global] Instance SubstIntro_all
+  (A : Type)
+  (staleA : Stale A)
+  (openA  : Open value A)
+  (substA : Subst value A)
+  (lcA    : Lc A)
+  (substOpenA  : @SubstOpen  A staleA openA substA lcA)
+  (substFreshA : @SubstFresh A staleA substA)
+  : @SubstIntro A staleA openA substA lcA.
+Proof.
+  unfold SubstIntro. intros e x w k Hx Hlc.
+  rewrite subst_open; auto.
+  ln_simpl; f_equal; hauto.
+Qed.
+
+Class SubstOpenVar A `{Stale aset A} `{Open value A} `{Subst value A} `{Lc A} := subst_open_var :
+forall x y (u: value) (e: A) (k: nat),
+    x <> y -> lc u -> {x := u} ({k ~> (vfvar y)} e) = ({k ~> (vfvar y)} ({x := u} e)).
+
+#[global] Instance SubstOpenVar_all
+  (A : Type)
+  (staleA : Stale A)
+  (openA  : Open value A)
+  (substA : Subst value A)
+  (lcA    : Lc A)
+  (subst_openA : @SubstOpen A staleA openA substA lcA)
+  : @SubstOpenVar A staleA openA substA lcA.
+Proof.
+  unfold SubstOpenVar. intros x y u e k Hxy Hlc.
+  rewrite subst_open; auto. ln_simpl; f_equal; hauto.
+Qed.
+Arguments SubstOpenVar_all /.
+
+Class SubstBody A `{Stale aset A} `{open: Open value A} `{Subst value A} `{lc : Lc A}:= subst_body :
+forall x (u: value) (e: A), body e -> lc_value u -> body ({x := u} e).
+
+#[global] Instance SubstBody_all
+  (A : Type)
+  (staleA : Stale A)
+  (openA  : Open value A)
+  (substA : Subst value A)
+  (lcA    : Lc A)
+  (substOpenVarA : @SubstOpenVar A staleA openA substA lcA)
+  (substLcA      : @SubstLc      A staleA substA lcA)
+  : @SubstBody A staleA openA substA lcA.
+Proof.
+  unfold SubstBody. intros x u e Hbody Hlc.
+  destruct Hbody as [L Hbody].
+  auto_exists_L; intros y Hy; repeat split; auto.
+  rewrite <- subst_open_var by set_solver.
+  apply subst_lc; auto. apply Hbody; my_set_solver.
+Qed.
+
+Class OpenLc A `{Stale aset A} `{Open value A} `{Lc A} := open_lc :
+forall (e: A) (u: value), body e -> lc u -> lc ({0 ~> u} e).
+
+#[global] Instance OpenLc_all
+  (A : Type)
+  (staleA : Stale A)
+  (openA  : Open value A)
+  (substA : Subst value A)
+  (lcA    : Lc A)
+  (substIntroA : @SubstIntro A staleA openA substA lcA)
+  (substLcA    : @SubstLc    A staleA substA lcA)
+  : @OpenLc A staleA openA lcA.
+Proof.
+  intros e u Hbody Hlc. destruct Hbody as [L Hbody].
+  pose_fresh_fv y.
+  erewrite <- subst_intro; auto. instantiate (1:= y).
+  apply subst_lc; auto. apply Hbody; my_set_solver.
+  my_set_solver.
+Qed.
+
+Class OpenWithFreshIncludeFv A `{Stale aset A} `{Open value A} `{Lc A} := open_with_fresh_include_fv :
+forall (x: atom) (e: A) (k: nat),
+    x # e -> ({[x]} ∪ stale e) ⊆ ({[x]} ∪ stale ({k ~> (vfvar x)} e)).
+
+#[global] Instance OpenWithFreshIncludeFv_tm : OpenWithFreshIncludeFv tm.
+Proof.
+  unfold OpenWithFreshIncludeFv.
+  intros x.
+  apply (tm_mutual_rec
+           (fun (e: value) => forall k, x # e -> ({[x]} ∪ stale e) ⊆ ({[x]} ∪ stale ({k ~> (vfvar x)} e)))
+           (fun (e: tm) => forall k, x # e -> ({[x]} ∪ stale e) ⊆ ({[x]} ∪ stale ({k ~> (vfvar x)} e)))
+        ); simpl; intros; auto; ln_simpl.
+    all:
+    repeat match goal with
+           | [H: context [{_ ~> _} ?e] |- context [{?k ~> _} ?e]] => specialize (H k)
+           | [H: context [{_ ~> _} ?e] |- context [{?k ~> _} ?e]] => specialize (H k)
+           | [H: ?P -> _ ⊆ _ |- _] => assert P as Htmp by fast_set_solver; specialize (H Htmp); try clear Htmp
+           end; repeat my_set_solver.
+Qed.
+Arguments OpenWithFreshIncludeFv_tm /.
+
+#[global] Instance OpenWithFreshIncludeFv_value : OpenWithFreshIncludeFv value.
+Proof.
+  unfold OpenWithFreshIncludeFv.
+  intros x.
+  apply (value_mutual_rec
+           (fun (e: value) => forall k, x # e -> ({[x]} ∪ stale e) ⊆ ({[x]} ∪ stale ({k ~> (vfvar x)} e)))
+           (fun (e: tm) => forall k, x # e -> ({[x]} ∪ stale e) ⊆ ({[x]} ∪ stale ({k ~> (vfvar x)} e)))
+        ); simpl; intros; auto; ln_simpl.
+    all:
+    repeat match goal with
+           | [H: context [{_ ~> _} ?e] |- context [{?k ~> _} ?e]] => specialize (H k)
+           | [H: context [{_ ~> _} ?e] |- context [{?k ~> _} ?e]] => specialize (H k)
+           | [H: ?P -> _ ⊆ _ |- _] => assert P as Htmp by fast_set_solver; specialize (H Htmp); try clear Htmp
+           end; repeat my_set_solver.
+Qed.
+Arguments OpenWithFreshIncludeFv_value /.
+
+(* Lemma for MNF *)
+
+Class LcImpliesBody A `{Open value A} `{Lc A} := lc_implies_body :
+forall (e: A), lc e -> body e.
+
+#[global] Instance LcImpliesBody_all
+    (A : Type)
+    `{stale: Stale aset A}
+    `{open: Open value A} `{lc: Lc A}
+    `{open_rec_lc: @OpenRecLc A stale open lc}
+: @LcImpliesBody A open lc.
+Proof.
+  unfold LcImpliesBody.
+  intros. exists ∅; intros; rewrite open_rec_lc; auto.
+Qed.
+Arguments LcImpliesBody_all /.
+
+(* Ltac lc_solver :=
+  repeat match goal with
+    | [ |- lc (treturn (vfvar _))] => constructor
+    | [ |- lc (tmatchb _ _ _)] => apply lc_tmatchb; (repeat split; auto)
+    | [ |- lc (tletapp _ _ _)] => rewrite letapp_lc_body; (repeat split; auto)
+    | [ |- lc (tleteffop _ _ _)] => rewrite leteffop_lc_body; (repeat split; auto)
+    | [ |- lc (tlete _ _)] => rewrite lete_lc_body; split; auto
+    | [ |- lc (treturn (vfix _ _))] => rewrite lc_fix_iff_body; auto
+    | [ |- lc (treturn (vlam _ _))] => rewrite lc_abs_iff_body; auto
+    | [H: lc (tlete _ ?e) |- body ?e ] => rewrite lete_lc_body in H; mydestr; auto
+    | [H: lc (tletapp _ _ ?e) |- body ?e ] => rewrite letapp_lc_body in H; mydestr; auto
+    | [H: lc (treturn (vlam _ ?e)) |- body ?e ] => rewrite lc_abs_iff_body in H; mydestr; auto
+    | [H: lc (treturn (vfix _ ?e)) |- body ?e ] => rewrite lc_fix_iff_body in H; mydestr; auto
+    | [H: lc (tletapp ?e _ _) |- lc (treturn ?e) ] => rewrite letapp_lc_body in H; mydestr; auto
+    | [H: lc (tletapp _ ?e _) |- lc (treturn ?e) ] => rewrite letapp_lc_body in H; mydestr; auto
+    | [H: lc ?e |- body ?e] => apply lc_implies_body_tm; auto
+    | [H: lc ?e |- lc (?e ^t^ _)] => rewrite open_rec_lc_tm; auto
+    | [|- body _ ] => eexists; auto_exists_L_intros
+    end. *)
+
+Class SubstAsCloseOpenAux A `{Stale aset A} `{Open value A} `{Close A} `{Subst value A} := subst_as_close_open_aux :
+forall (x: atom) (u: value) (e: A) (k: nat),
+    {k ~> u} e = e ->
+    {k ~> u} ({k <~ x} e) = {x := u} e.
+
+#[global] Instance SubstAsCloseOpenAux_tm : SubstAsCloseOpenAux tm.
+Proof.
+  unfold SubstAsCloseOpenAux.
+  intros x u.
+  apply (tm_mutual_rec
+           (fun (e: value) => forall k, {k ~> u} e = e -> {k ~> u} ({k <~ x} e) = {x := u} e)
+           (fun (e: tm) => forall k, {k ~> u} e = e -> {k ~> u} ({k <~ x} e) = {x := u} e)
+        ); ln_simpl; intros; rewrite_by_set_solver2; eauto. 
+  - repeat ln_simpl; hauto.
+Qed.
+Arguments SubstAsCloseOpenAux_tm /.
+
+#[global] Instance SubstAsCloseOpenAux_value : SubstAsCloseOpenAux value.
+Proof.
+  unfold SubstAsCloseOpenAux.
+  intros x u.
+  apply (value_mutual_rec
+           (fun (e: value) => forall k, {k ~> u} e = e -> {k ~> u} ({k <~ x} e) = {x := u} e)
+           (fun (e: tm) => forall k, {k ~> u} e = e -> {k ~> u} ({k <~ x} e) = {x := u} e)
+        ); ln_simpl; intros; rewrite_by_set_solver2; eauto. 
+  - repeat ln_simpl; hauto.
+Qed.
+Arguments SubstAsCloseOpenAux_value /.
+
+Class SubstAsCloseOpen A `{Stale aset A} `{Open value A} `{Close A} `{Subst value A} `{Lc A} := subst_as_close_open :
+forall (x: atom) (u: value) (e: A),
+    lc e -> {0 ~> u} ({0 <~ x} e) = {x := u} e.
+
+#[global] Instance SubstAsCloseOpen_all
+  (A : Type)
+  (staleA : Stale A)
+  (openA  : Open value A)
+  (closeA : Close A)
+  (substA : Subst value A)
+  (lcA    : Lc A)
+  (substAsCloseOpenAuxA : @SubstAsCloseOpenAux A staleA openA closeA substA)
+  (openRecLcA           : @OpenRecLc           A staleA openA lcA)
+  : @SubstAsCloseOpen A staleA openA closeA substA lcA.
+Proof.
+  unfold SubstAsCloseOpen.
+  intros x u e Hlc. eapply subst_as_close_open_aux; auto.
+Qed.
+Arguments SubstAsCloseOpen_all /.
+
+Class CloseFreshRec A `{Stale aset A} `{Close A} := close_fresh_rec :
+forall (x: atom) (e: A) (k: nat), x # e -> { k <~ x} e = e.
+
+#[global] Instance CloseFreshRec_tm : CloseFreshRec tm.
+Proof.
+  unfold CloseFreshRec.
+  intros x.
+  apply (tm_mutual_rec
+           (fun (v: value) => forall (k: nat), x # v -> { k <~ x} v = v)
+           (fun (e: tm) => forall (k: nat), x # e -> { k <~ x} e = e)
+        ); simpl; intros; auto; ln_simpl; rewrite_by_set_solver2; auto.
+  - my_set_solver.
+Qed.
+Arguments CloseFreshRec_tm /.
+
+#[global] Instance CloseFreshRec_value : CloseFreshRec value.
+Proof.
+  unfold CloseFreshRec.
+  intros x.
+  apply (value_mutual_rec
+           (fun (v: value) => forall (k: nat), x # v -> { k <~ x} v = v)
+           (fun (e: tm) => forall (k: nat), x # e -> { k <~ x} e = e)
+        ); simpl; intros; auto; ln_simpl; rewrite_by_set_solver2; auto.
+  - my_set_solver.
+Qed.
+Arguments CloseFreshRec_value /.
+
+Class SubstClose A `{Stale aset A} `{Open value A} `{Close A} `{Subst value A} := subst_close :
+∀ (x y: atom) (u: value), x # u -> x <> y ->
+                        forall (e: A) k, {k <~ x} ({y := u } e) = {y := u } ({k <~ x} e).
+
+#[global] Instance SubstClose_tm: SubstClose tm.
+Proof.
+  unfold SubstClose.
+  intros x y u Hux Hxy. apply (tm_mutual_rec
+           (fun (e: value) => forall (k: nat), {k <~ x} ({y := u } e) = {y := u } ({k <~ x} e))
+           (fun (e: tm) => forall (k: nat), {k <~ x} ({y := u } e) = {y := u } ({k <~ x} e))
+        ); simpl; intros; auto; ln_simpl; rewrite_by_set_solver2; auto;
+  try (ln_simpl; hauto).
+  - ln_simpl; auto. rewrite close_fresh_rec; auto. hauto.
+Qed.
+Arguments SubstClose_tm /.
+
+#[global] Instance SubstClose_value: SubstClose value.
+Proof.
+  unfold SubstClose.
+  intros x y u Hux Hxy. apply (value_mutual_rec
+           (fun (e: value) => forall (k: nat), {k <~ x} ({y := u } e) = {y := u } ({k <~ x} e))
+           (fun (e: tm) => forall (k: nat), {k <~ x} ({y := u } e) = {y := u } ({k <~ x} e))
+        ); simpl; intros; auto; ln_simpl; rewrite_by_set_solver2; auto;
+  try (ln_simpl; hauto).
+  - ln_simpl; auto. rewrite close_fresh_rec; auto. hauto.
+Qed.
+Arguments SubstClose_value /.
+
+Class SubstCommute A `{Stale aset A} `{Subst value A} := subst_commute :
+forall (x y: atom) (u_x u_y: value) (e: A),
+    x <> y -> x # u_y -> y # u_x ->
+    {x := u_x } ({y := u_y } e) = {y := u_y } ({x := u_x } e).
+
+#[global] Instance SubstCommute_tm: SubstCommute tm.
+Proof.
+  unfold SubstCommute.
+  intros x y u_x u_y e Hxy Hxuy Hyux. 
+  apply (tm_mutual_rec
+           (fun (e: value) => {x := u_x } ({y := u_y } e) = {y := u_y } ({x := u_x } e))
+           (fun (e: tm) => {x := u_x } ({y := u_y } e) = {y := u_y } ({x := u_x } e))
+        ); simpl; intros; auto; ln_simpl; auto;
+  try solve [f_equal; auto];
+  try solve [ln_simpl; try hauto; rewrite subst_fresh; auto].
+Qed.
+Arguments SubstCommute_tm /.
+
+#[global] Instance SubstCommute_value: SubstCommute value.
+Proof.
+  unfold SubstCommute.
+  intros x y u_x u_y e Hxy Hxuy Hyux. 
+  apply (value_mutual_rec
+           (fun (e: value) => {x := u_x } ({y := u_y } e) = {y := u_y } ({x := u_x } e))
+           (fun (e: tm) => {x := u_x } ({y := u_y } e) = {y := u_y } ({x := u_x } e))
+        ); simpl; intros; auto; ln_simpl; auto;
+  try solve [f_equal; auto];
+  try solve [ln_simpl; try hauto; rewrite subst_fresh; auto].
+Qed.
+Arguments SubstCommute_value /.
+
+Class SubstShadow A `{Stale aset A} `{Open value A} `{Close A} `{Subst value A} := subst_shadow :
+forall (x z: atom) (u: value) (e: A),
+    x # e -> {x := u } ({z := (vfvar x) } e) = {z := u } e.
+
+#[global] Instance SubstShadow_tm: SubstShadow tm.
+Proof.
+  unfold SubstShadow.
+  intros x z u e Hx. apply (tm_mutual_rec
+           (fun (e: value) => x # e -> {x := u } ({z := (vfvar x) } e) = {z := u } e)
+           (fun (e: tm) => x # e -> {x := u } ({z := (vfvar x) } e) = {z := u } e)
+        ); intros; auto; ln_simpl; rewrite_by_set_solver2; eauto;
+  try solve [f_equal; ln_simpl; my_set_solver].
+Qed.
+Arguments SubstShadow_tm /.
+
+#[global] Instance SubstShadow_value: SubstShadow value.
+Proof.
+  unfold SubstShadow.
+  intros x z u e Hx. apply (value_mutual_rec
+           (fun (e: value) => x # e -> {x := u } ({z := (vfvar x) } e) = {z := u } e)
+           (fun (e: tm) => x # e -> {x := u } ({z := (vfvar x) } e) = {z := u } e)
+        ); intros; auto; ln_simpl; rewrite_by_set_solver2; eauto;
+  try solve [f_equal; ln_simpl; my_set_solver].
+Qed.
+Arguments SubstShadow_value /.
+
+Class SubstSubst A `{Stale aset A} `{Open value A} `{Close A} `{Subst value A} := subst_subst :
+forall (x : atom) (u_x : value) (y : atom) (u_y: value) (e: A),
+    x ≠ y → y # u_x →
+    {x := u_x } ({y := u_y } e) = {y := {x := u_x } u_y } ({x := u_x } e).
+
+#[global] Instance SubstSubst_tm: SubstSubst tm.
+Proof.
+  unfold SubstSubst.
+  intros x u_x y u_y e Hxy Hyux. apply (tm_mutual_rec
+           (fun (e: value) => {x := u_x } ({y := u_y } e) = {y := {x := u_x } u_y } ({x := u_x } e))
+           (fun (e: tm) => {x := u_x } ({y := u_y } e) = {y := {x := u_x } u_y } ({x := u_x } e))
+        ); intros; ln_simpl; auto; rewrite_by_set_solver2; auto; fold_syntax_class;
+  try solve [ln_simpl; hauto].
+  - ln_simpl; try hauto. rewrite subst_fresh; auto.
+Qed.
+Arguments SubstSubst_tm /.
+
+#[global] Instance SubstSubst_value: SubstSubst value.
+Proof.
+  unfold SubstSubst.
+  intros x u_x y u_y e Hxy Hyux. apply (value_mutual_rec
+           (fun (e: value) => {x := u_x } ({y := u_y } e) = {y := {x := u_x } u_y } ({x := u_x } e))
+           (fun (e: tm) => {x := u_x } ({y := u_y } e) = {y := {x := u_x } u_y } ({x := u_x } e))
+        ); intros; ln_simpl; auto; rewrite_by_set_solver2; auto; fold_syntax_class;
+  try solve [ln_simpl; hauto].
+  - ln_simpl; try hauto. rewrite subst_fresh; auto.
+Qed.
+Arguments SubstSubst_value /.
+
+Class FvOfSubst A `{Stale aset A} `{Open value A} `{Close A} `{Subst value A} := fv_of_subst :
+forall x (u: value) (e: A), stale ({x := u } e) ⊆ (stale e ∖ {[x]}) ∪ stale u.
+
+#[global] Instance FvOfSubst_tm: FvOfSubst tm.
+Proof.
+  unfold FvOfSubst.
+  intros x u e. apply (tm_mutual_rec
+           (fun (e: value) => stale ({x := u } e) ⊆ stale e ∖ {[x]} ∪ stale u)
+           (fun (e: tm) => stale ({x := u } e) ⊆ stale e ∖ {[x]} ∪ stale u)
+        ); intros; ln_simpl; auto; rewrite_by_set_solver2; auto; fold_syntax_class;
+  try solve [ln_simpl; set_solver].
+Qed.
+Arguments FvOfSubst_tm /.
+
+#[global] Instance FvOfSubst_value: FvOfSubst value.
+Proof.
+  unfold FvOfSubst.
+  intros x u e. apply (value_mutual_rec
+           (fun (e: value) => stale ({x := u } e) ⊆ stale e ∖ {[x]} ∪ stale u)
+           (fun (e: tm) => stale ({x := u } e) ⊆ stale e ∖ {[x]} ∪ stale u)
+        ); intros; ln_simpl; auto; rewrite_by_set_solver2; auto; fold_syntax_class;
+  try solve [ln_simpl; set_solver].
+Qed.
+Arguments FvOfSubst_value /.
+
+Class FvOfSubstClosed A `{Stale aset A} `{Subst value A} := fv_of_subst_closed :
+forall x (u: value) (e: A),
+    stale u ≡ ∅ ->
+    stale ({x := u } e) = (stale e ∖ {[x]}).
+
+#[global] Instance FvOfSubstClosed_tm: FvOfSubstClosed tm.
+Proof.
+  unfold FvOfSubstClosed.
+  intros x u.
+  apply (tm_mutual_rec
+           (fun (e: value) =>
+              fv_value u ≡ ∅ -> fv_value ({x := u } e) = fv_value e ∖ {[x]})
+           (fun (e: tm) =>
+              fv_value u ≡ ∅ -> fv_tm ({x := u } e) = fv_tm e ∖ {[x]})
+        ); simpl; intros; auto; repeat ln_simpl; my_set_solver.
+Qed.
+Arguments FvOfSubstClosed_tm /.
+
+#[global] Instance FvOfSubstClosed_value: FvOfSubstClosed value.
+Proof.
+  unfold FvOfSubstClosed.
+  intros x u.
+  apply (value_mutual_rec
+           (fun (e: value) =>
+              fv_value u ≡ ∅ -> fv_value ({x := u } e) = fv_value e ∖ {[x]})
+           (fun (e: tm) =>
+              fv_value u ≡ ∅ -> fv_tm ({x := u } e) = fv_tm e ∖ {[x]})
+        ); simpl; intros; auto; repeat ln_simpl; my_set_solver.
+Qed.
+Arguments FvOfSubstClosed_value /.
+
+Lemma lc_tletapp: forall (v x: value), lc v -> lc x -> lc (tletapp v x (treturn (vbvar 0))).
+Proof.
+  intros. auto_exists_L; ln_simpl; intros; lc_solver1.
+Qed.
+
+Global Hint Resolve lc_tletapp: core.
+
+Lemma body_tletapp_0: forall (v: value), lc v -> body (tletapp v (vbvar 0) (treturn (vbvar 0))).
+Proof.
+  intros. auto_exists_L; intros. ln_simpl.
+  rewrite open_rec_lc; eauto.
+  apply lc_tletapp; hauto.
+Qed.
+
+Global Hint Resolve body_tletapp_0: core.
+
+Class OpenSubstSame A `{Stale aset A} `{Open value A} `{Subst value A} := open_subst_same :
+forall (x: atom) (y: value) (e: A) (k: nat), x # e -> {x := y } ({k ~> (vfvar x)} e) = {k ~> y} e.
+
+#[global] Instance OpenSubstSame_tm: OpenSubstSame tm.
+Proof.
+  unfold OpenSubstSame.
+  intros x y. apply (tm_mutual_rec
+  (fun (e: value) => forall k,
+     x # e -> {x := y } ({k ~> (vfvar x)} e) = {k ~> y} e)
+  (fun (e: tm) => forall k,
+     x # e -> {x := y } ({k ~> (vfvar x)} e) = {k ~> y} e)
+); intros; ln_simpl; auto; rewrite_by_set_solver2; auto; fold_syntax_class;
+  try solve [ln_simpl; hauto].
+  - set_solver.
+Qed.
+Arguments OpenSubstSame_tm /.
+
+#[global] Instance OpenSubstSame_value: OpenSubstSame value.
+Proof.
+  unfold OpenSubstSame.
+  intros x y. apply (value_mutual_rec
+                   (fun (e: value) => forall k,
+                      x # e -> {x := y } ({k ~> (vfvar x)} e) = {k ~> y} e)
+                   (fun (e: tm) => forall k,
+                      x # e -> {x := y } ({k ~> (vfvar x)} e) = {k ~> y} e)
+                ); intros; ln_simpl; auto; rewrite_by_set_solver2; auto; fold_syntax_class;
+  try solve [ln_simpl; hauto].
+  - set_solver.
+Qed.
+Arguments OpenSubstSame_value /.
+
+Lemma body_vlam_eq: forall e T1 T2,
+    body (vlam T1 e) <-> body (vlam T2 e).
+Proof.
+  apply (tm_mutual_rec
+                   (fun (e: value) => forall T1 T2, body (vlam T1 (treturn e)) <-> body (vlam T2 (treturn e)))
+                   (fun (e: tm) => forall T1 T2, body (vlam T1 e) <-> body (vlam T2 e))
+                ); split; ln_simpl; intros; auto;
+    repeat match goal with
+    | [H: body ( (vlam _ _)) |- _ ] => invclear H
+    | [|- body ( (vlam _ _))] => auto_exists_L; intros a; intros; specialize_with a
+    | [H: context [( (vlam _ _)) ^^ _] |- _ ] => ln_simpl
+    | [|- context [( (vlam _ _)) ^^ _] ] => ln_simpl
+    | [H: lc ( (vlam _ _)) |- _ ] => rewrite lc_abs_iff_body in H; auto
+    | [|- lc ( (vlam _ _))] => rewrite lc_abs_iff_body; auto
+    end.
+Qed.
+
+Class CloseRmFv A `{Stale aset A} `{Close A} := close_rm_fv :
+forall (x: atom) (e: A) (k: nat), x # ({k <~ x} e).
+
+#[global] Instance CloseRmFv_tm: CloseRmFv tm.
+Proof.
+  unfold CloseRmFv.
+  intros x. apply (tm_mutual_rec
+                   (fun (e: value) => forall k, x # ({k <~ x} e))
+                   (fun (e: tm) => forall k, x # ({k <~ x} e))
+                ); intros; ln_simpl; auto; rewrite_by_set_solver2; auto; fold_syntax_class;
+  try solve [ln_simpl; my_set_solver].
+Qed.
+Arguments CloseRmFv_tm /.
+
+#[global] Instance CloseRmFv_value: CloseRmFv value.
+Proof.
+  unfold CloseRmFv.
+  intros x.
+  apply (value_mutual_rec
+                   (fun (e: value) => forall (k: nat), x # ({k <~ x} e))
+                   (fun (e: tm) => forall (k: nat), x # ({k <~ x} e))
+                ); intros; ln_simpl; auto; rewrite_by_set_solver2; auto; fold_syntax_class;
+  try solve [ln_simpl; my_set_solver].
+Qed.
+Arguments CloseRmFv_value /.
+
+Class CloseThenSubstSame A `{Stale aset A} `{Close A} `{Subst value A} := close_then_subst_same :
+forall (x: atom) (v_x: value) (e: A), ({x := v_x } (x \\ e)) = (x \\ e).
+
+#[global] Instance CloseThenSubstSame_all
+  (A : Type)
+  (staleA : Stale A)
+  (closeA : Close A)
+  (substA : Subst value A)
+  (substFreshA : @SubstFresh   A staleA substA)
+  (closeRmFvA  : @CloseRmFv    A staleA closeA)
+  : @CloseThenSubstSame A staleA closeA substA.
+Proof.
+  unfold CloseThenSubstSame. hauto.
+Qed.
+Arguments CloseThenSubstSame_all /.
+
+Class SubstOpenClosed A `{Stale aset A} `{Open value A} `{Subst value A} `{Lc A} := subst_open_closed :
+forall (e :A) (x : atom) (u w : value) (k : nat),
+    stale u ≡ ∅ ->
+    lc w → {x := w } ({k ~> u} e) = {k ~> u} ({x := w } e).
+
+#[global] Instance SubstOpenClosed_all
+  (A : Type)
+  (staleA : Stale A)
+  (openA  : Open value A)
+  (substA : Subst value A)
+  (lcA    : Lc A)
+  (substOpenA : @SubstOpen A staleA openA substA lcA)
+  : @SubstOpenClosed A staleA openA substA lcA.
+Proof.
+  unfold SubstOpenClosed. intros. 
+  rewrite subst_open; auto.
+  rewrite SubstFresh_value; eauto. set_solver.
+Qed.
+Arguments SubstOpenClosed_all /.
+
+Class BodyLcAfterClose A `{Stale aset A} `{Open value A} `{Close A} `{Lc A} := body_lc_after_close :
+forall (x: atom) (e: A), lc e -> body ({0 <~ x} e).
+
+#[global] Instance BodyLcAfterClose_all
+  (A : Type)
+  (staleA : Stale A)
+  (openA  : Open value A)
+  (closeA : Close A)
+  (substA : Subst value A)
+  (lcA    : Lc A)
+  (substAsCloseOpenA : @SubstAsCloseOpen A staleA openA closeA substA lcA)
+  (substLcA          : @SubstLc         A staleA substA lcA)
+  : @BodyLcAfterClose A staleA openA closeA lcA.
+Proof.
+  unfold BodyLcAfterClose. 
+  intros. unfold body. auto_exists_L. intros.
+  rewrite subst_as_close_open; auto.
+  apply subst_lc; hauto.
+Qed.
+Arguments BodyLcAfterClose_all /.
+
+Class LcFreshVarImpliesBody A `{Stale aset A} `{Open value A} `{Close A} `{Lc A} := lc_fresh_var_implies_body :
+forall (e: A) (x: atom), x # e -> lc (e ^^ (vfvar x)) -> body e.
+
+#[global] Instance LcFreshVarImpliesBody_all
+  (A : Type)
+  (staleA : Stale A)
+  (openA  : Open value A)
+  (closeA : Close A)
+  (lcA    : Lc A)
+  (bodyLcAfterCloseA : @BodyLcAfterClose A staleA openA closeA lcA)
+  (closeOpenVarA     : @CloseOpenVar     A staleA openA closeA)
+  : @LcFreshVarImpliesBody A staleA openA closeA lcA.
+Proof.
+  unfold LcFreshVarImpliesBody. intros x e Hx Hlc.
+  eapply (body_lc_after_close) in Hlc; eauto. rewrite close_open_var in Hlc; auto.
+Qed.
+Arguments LcFreshVarImpliesBody_all /.
+
+Class OpenNotInEq A `{Stale aset A} `{Open value A} := open_not_in_eq :
+forall (x: atom) (e: A) (k: nat), x # ({k ~> (vfvar x)} e) -> {k ~> (vfvar x)} e = e.
+
+#[global] Instance OpenNotInEq_tm: OpenNotInEq tm.
+Proof.
+  unfold OpenNotInEq. intros x.
+  apply (tm_mutual_rec
+                   (fun (e: value) => forall k, x # ({k ~> (vfvar x)} e) -> {k ~> (vfvar x)} e = e)
+                   (fun (e: tm) => forall k, x # ({k ~> (vfvar x)} e) -> {k ~> (vfvar x)} e = e)
+                ); intros; ln_simpl; auto; rewrite_by_set_solver2; auto; fold_syntax_class;
+  try solve [ln_simpl; my_set_solver].
+Qed.
+Arguments OpenNotInEq_tm /.
+
+#[global] Instance OpenNotInEq_value: OpenNotInEq value.
+Proof.
+  unfold OpenNotInEq. intros x.
+  apply (value_mutual_rec
+                   (fun (e: value) => forall k, x # ({k ~> (vfvar x)} e) -> {k ~> (vfvar x)} e = e)
+                   (fun (e: tm) => forall k, x # ({k ~> (vfvar x)} e) -> {k ~> (vfvar x)} e = e)
+                ); intros; ln_simpl; auto; rewrite_by_set_solver2; auto; fold_syntax_class;
+  try solve [ln_simpl; my_set_solver].
+Qed.
+Arguments OpenNotInEq_value /.
+
+Class LcSubst A `{Stale aset A} `{Open value A} `{Subst value A} `{Lc A} := lc_subst :
+forall (x: atom) (u: value) (e: A), lc ({x := u} e) -> lc_value u -> lc e.
+
+#[global] Instance LcSubst_tm : LcSubst tm.
+Proof.
+  pose SubstOpenVar_all.
+  pose SubstOpen_tm. 
+  pose SubstOpen_value.
+  unfold LcSubst. intros x u e Hlc Hu.
+  remember ({x := u} e) as e'.
+  generalize dependent e.
+  generalize dependent e'.
+  apply (lc_tm_mutual_rec
+           (fun (e': value) _ => ∀ e : value, e' = {x := u} (e) → lc e)
+           (fun (e': tm) _ => ∀ e : tm, e' = {x := u} (e) → lc e)
+        ); intros;
+      match goal with
+      | H : _ = {_:=_} ?e |- _ => destruct e; ln_simpl; simplify_eq
+      end;
+  try solve [ lc_solver1; hauto].
+all: lc_solver1; econstructor; eauto;
+let x := fresh "x" in
+let acc := collect_stales tt in instantiate (1 := acc); intros x **; simpl;
+repeat specialize_with x;
+rewrite <- @subst_open_var with (H := stale) (H2:= lc) in *; eauto; my_set_solver.
+Qed.
+Arguments LcSubst_tm /.
+
+#[global] Instance LcSubst_value : LcSubst value.
+Proof.
+  pose SubstOpenVar_all.
+  pose SubstOpen_tm. 
+  pose SubstOpen_value.
+  unfold LcSubst. intros x u e Hlc Hu.
+  remember ({x := u} e) as e'.
+  generalize dependent e.
+  generalize dependent e'.
+  apply (lc_value_mutual_rec
+           (fun (e': value) _ => ∀ e : value, e' = {x := u} (e) → lc e)
+           (fun (e': tm) _ => ∀ e : tm, e' = {x := u} (e) → lc e)
+        ); intros;
+      match goal with
+      | H : _ = {_:=_} ?e |- _ => destruct e; ln_simpl; simplify_eq
+      end;
+  try solve [ lc_solver1; hauto].
+all: lc_solver1; econstructor; eauto;
+let x := fresh "x" in
+let acc := collect_stales tt in instantiate (1 := acc); intros x **; simpl;
+repeat specialize_with x;
+rewrite <- @subst_open_var with (H := stale) (H2:= lc) in *; eauto; my_set_solver.
+Qed.
+Arguments LcSubst_value /.
+
+Class OpenSwap A `{Stale aset A} `{Open value A} := open_swap :
+forall (t: A) i j (u v: value),
+    lc u ->
+    lc v ->
+    i <> j ->
+    {i ~> v} ({j ~> u} t) = {j ~> u} ({i ~> v} t).
+
+#[global] Instance OpenSwap_tm: OpenSwap tm.
+Proof.
+  unfold OpenSwap.
+  apply (tm_mutual_rec
+                   (fun (t: value) => forall i j (u v: value),
+                      lc u ->
+                      lc v ->
+                      i <> j ->
+                      {i ~> v} ({j ~> u} t) = {j ~> u} ({i ~> v} t))
+                   (fun (t: tm) => forall i j (u v: value),
+                      lc u ->
+                      lc v ->
+                      i <> j ->
+                      {i ~> v} ({j ~> u} t) = {j ~> u} ({i ~> v} t))
+                ); intros; ln_simpl; auto; fold_syntax_class;
+  try solve [ln_simpl; f_equal; hauto].
+  all: ln_simpl; try hauto; rewrite open_rec_lc; hauto.
+Qed.
+Arguments OpenSwap_tm /.
+
+#[global] Instance OpenSwap_value: OpenSwap value.
+Proof.
+  unfold OpenSwap.
+  apply (value_mutual_rec
+                   (fun (t: value) => forall i j (u v: value),
+                      lc u ->
+                      lc v ->
+                      i <> j ->
+                      {i ~> v} ({j ~> u} t) = {j ~> u} ({i ~> v} t))
+                   (fun (t: tm) => forall i j (u v: value),
+                      lc u ->
+                      lc v ->
+                      i <> j ->
+                      {i ~> v} ({j ~> u} t) = {j ~> u} ({i ~> v} t))
+                ); intros; ln_simpl; auto; fold_syntax_class;
+  try solve [ln_simpl; f_equal; hauto].
+  all: ln_simpl; try hauto; rewrite open_rec_lc; hauto.
+Qed.
+Arguments OpenSwap_value /.
+
+Class OpenLcRespect A `{Stale aset A} `{Open value A} `{Lc A} := open_lc_respect :
+forall (t: A) (u v : value) (k: nat),
+    lc ({k ~> u} t) ->
+    lc u ->
+    lc v ->
+    lc ({k ~> v} t).
+
+#[global] Instance OpenLcRespect_tm: OpenLcRespect tm.
+Proof.
+  unfold OpenLcRespect.
+  intros * H. remember ({k ~> u} t) as t'.
+  generalize dependent t. revert k.
+  apply (lc_tm_mutual_rec
+           (fun (t': value) _ => ∀ (k : nat) (t : value), t' = {k ~> u} t → lc u → lc v → lc {k ~> v} (t))
+           (fun (t': tm) _ => ∀ (k : nat) (t : tm), t' = {k ~> u} t → lc u → lc v → lc {k ~> v} t)
+        ); intros;
+      repeat match goal with
+      | H : _ = {_ ~> _} ?t |- _ => destruct t; ln_simpl; simplify_eq
+      end;
+  try solve [ lc_solver1; hauto].
+all: lc_solver1; econstructor; eauto;
+let x := fresh "x" in
+let acc := collect_stales tt in instantiate (1 := acc); intros x **; simpl;
+repeat specialize_with x; fold_syntax_class;
+rewrite open_swap in *; eauto; lc_solver1.
+Qed.
+Arguments OpenLcRespect_tm /.
+
+#[global] Instance OpenLcRespect_value: OpenLcRespect value.
+Proof.
+  unfold OpenLcRespect.
+  intros * H. remember ({k ~> u} t) as t'.
+  generalize dependent t. revert k.
+  apply (lc_value_mutual_rec
+           (fun (t': value) _ => ∀ (k : nat) (t : value), t' = {k ~> u} t → lc u → lc v → lc {k ~> v} t)
+           (fun (t': tm) _ => ∀ (k : nat) (t : tm), t' = {k ~> u} t → lc u → lc v → lc {k ~> v} t)
+        ); intros;
+      repeat match goal with
+      | H : _ = {_ ~> _} ?t |- _ => destruct t; ln_simpl; simplify_eq
+      end;
+  try solve [ lc_solver1; hauto].
+all: lc_solver1; econstructor; eauto;
+let x := fresh "x" in
+let acc := collect_stales tt in instantiate (1 := acc); intros x **; simpl;
+repeat specialize_with x; fold_syntax_class;
+rewrite open_swap in *; eauto; lc_solver1.
+Qed.
+Arguments OpenLcRespect_value /.
+
+Class OpenIdemp A `{Stale aset A} `{Open value A} := open_idemp :
+forall (t: A) (u v: value) (k: nat),
+    lc v ->
+    {k ~> u} ({k ~> v} t) = ({k ~> v} t).
+
+#[global] Instance OpenIdemp_tm: OpenIdemp tm.
+Proof.
+  unfold OpenIdemp.
+  apply (tm_mutual_rec
+                   (fun (t: value) => forall (u v: value) (k: nat),
+                      lc v ->
+                      {k ~> u} ({k ~> v} t) = ({k ~> v} t))
+                   (fun (t: tm) => forall (u v: value) (k: nat),
+                      lc v ->
+                      {k ~> u} ({k ~> v} t) = ({k ~> v} t))
+                ); intros; ln_simpl; f_equal; auto; fold_syntax_class;
+  try solve [ln_simpl; f_equal; hauto].
+  - rewrite open_rec_lc; hauto.
+Qed.
+Arguments OpenIdemp_tm /.
+
+#[global] Instance OpenIdemp_value: OpenIdemp value.
+Proof.
+  unfold OpenIdemp.
+  apply (value_mutual_rec
+                   (fun (t: value) => forall (u v: value) (k: nat),
+                      lc v ->
+                      {k ~> u} ({k ~> v} t) = ({k ~> v} t))
+                   (fun (t: tm) => forall (u v: value) (k: nat),
+                      lc v ->
+                      {k ~> u} ({k ~> v} t) = ({k ~> v} t))
+                ); intros; ln_simpl; f_equal; auto; fold_syntax_class;
+  try solve [ln_simpl; f_equal; hauto].
+  - rewrite open_rec_lc; hauto.
+Qed.
+Arguments OpenIdemp_value /.
+
+Global Hint Resolve lc_fresh_var_implies_body: core.
