LocallyNameless/QualifierLc.v
@@ -1,0 +1,447 @@
+From stdpp Require Import mapset.
+From stdpp Require Import natmap.
+From stdpp Require Import fin vector.
+From Stdlib Require Classical_Prop.
+From CT.Syntax Require Import Syntax.
+From CT.LocallyNameless Require Import LangLc.
+
+Import BaseDef.
+Import Lang.
+Import Primitives.
+Import Qualifier.
+Import MyTactics.
+
+#[global] Instance SubstCommute_qualifier: SubstCommute qualifier.
+Proof.
+  unfold SubstCommute.
+  intros x u_x y u_y ϕ Hxy Hxuy Hyux.
+  destruct ϕ.
+  ln_simpl.
+  f_equal.
+  rewrite !Vector.map_map.
+  apply Vector.map_ext. ln_simpl.
+  intros; rewrite subst_commute; eauto.
+Qed.
+Arguments subst_commute /.
+
+#[global] Instance SubstFresh_qualifier: SubstFresh qualifier.
+Proof.
+  unfold SubstFresh.
+  intros ϕ x u Hx.
+  destruct ϕ.
+  ln_simpl.
+  f_equal.
+  clear prop.
+  induction vals; simpl in *; eauto.
+  f_equal.
+  apply subst_fresh. my_set_solver.
+  auto_apply. my_set_solver.
+Qed.
+Arguments SubstFresh_qualifier /.
+
+#[global] Instance OpenFv_qualifier: OpenFv qualifier.
+Proof.
+  unfold OpenFv.
+  intros ϕ v k.
+  destruct ϕ.
+  ln_simpl. clear. induction vals; ln_simpl. easy.
+  etrans. apply union_mono. apply open_fv.
+  reflexivity. my_set_solver.
+Qed.
+Arguments OpenFv_qualifier /.
+
+#[global] Instance OpenFvPrime_qualifier: OpenFvPrime qualifier.
+Proof.
+  unfold OpenFvPrime.
+  intros ϕ v k.
+  destruct ϕ.
+  ln_simpl. clear. induction vals; ln_simpl. easy.
+  apply union_mono; eauto. apply open_fv'.
+Qed.
+Arguments OpenFvPrime_qualifier /.
+
+Lemma lc_qualifier_and q1 q2 :
+  lc_qualifier q1 -> lc_qualifier q2 ->
+  lc_qualifier (q1 & q2).
+Proof.
+  inversion 1. inversion 1. subst.
+  simpl. constructor.
+  rewrite Vector.to_list_Forall in *.
+  rewrite Vector.to_list_append.
+  apply Forall_app. eauto.
+Qed.
+
+Lemma vector_map_app {A B: Type} (f: A -> B) {n1 n2: nat} (vec1: vec A n1) (vec2: vec A n2):
+  vmap f (vec1 +++ vec2) = vmap f vec1 +++ vmap f vec2.
+Proof.
+  induction vec1; simpl; eauto.
+  f_equal. eauto.
+Qed.
+
+Lemma qualifier_and_open k v q1 q2 :
+  {k ~> v} (q1 & q2) = ({k ~> v} q1) & ({k ~> v} q2).
+Proof.
+  destruct q1, q2. ln_simpl. f_equal. apply vector_map_app.
+Qed.
+
+Lemma qualifier_and_subst x v q1 q2 :
+  {x := v} (q1 & q2) = ({x := v} q1) & ({x := v} q2).
+Proof.
+  destruct q1, q2. ln_simpl. f_equal. apply vector_map_app.
+Qed.
+
+Lemma qualifier_and_fv q1 q2 :
+  stale (q1 & q2) = stale q1 ∪ stale q2.
+Proof.
+  destruct q1, q2. ln_simpl.
+  clear.
+  induction vals; ln_simpl. my_set_solver.
+  rewrite IHvals. my_set_solver.
+Qed.
+
+Lemma denote_vals_app {n1 n2} (vals1 : vec value n1) (vals2 : vec value n2) :
+  denote_vals (vals1 +++ vals2) =
+    match denote_vals vals1, denote_vals vals2 with
+    | Some v1, Some v2 => Some (v1 +++ v2)
+    | _, _ => None
+    end.
+Proof.
+  induction vals1; simpl; qauto.
+Qed.
+
+Lemma denote_qualifier_and q1 q2 :
+  denote_qualifier (q1 & q2) <-> denote_qualifier q1 /\ denote_qualifier q2.
+Proof.
+  destruct q1, q2. simpl.
+  rewrite denote_vals_app.
+  case_split; try qauto.
+  case_split; try qauto.
+  rewrite Vector.splitat_append. eauto.
+Qed.
+
+#[global] Instance OpenSubstSame_qualifier: OpenSubstSame qualifier.
+Proof.
+  unfold OpenSubstSame.
+  intros x y ϕ k H.
+  destruct ϕ. ln_simpl.
+  f_equal. clear - H.
+  induction vals; cbn; eauto.
+  cbn in H.
+  f_equal. fold_syntax_class. apply open_subst_same. my_set_solver.
+  apply IHvals. my_set_solver.
+Qed.
+Arguments OpenSubstSame_qualifier /.
+
+#[global] Instance SubstOpen_qualifier: SubstOpen qualifier.
+Proof.
+  unfold SubstOpen.
+  intros ϕ x u w k H.
+  destruct ϕ. cbn. intros.
+  f_equal.
+  rewrite !Vector.map_map.
+  apply Vector.map_ext. fold_syntax_class.
+  intros.  
+  rewrite subst_open; eauto.
+Qed.
+Arguments SubstOpen_qualifier /.
+
+#[global] Instance SubstOpenClosed_qualifier: SubstOpenClosed qualifier.
+Proof.
+  unfold SubstOpenClosed.
+  intros ϕ x u w k H Hlc.
+  rewrite subst_open; auto.
+  rewrite (subst_fresh); eauto. set_solver.
+Qed.
+Arguments SubstOpenClosed_qualifier /.
+
+#[global] Instance SubstLc_qualifier: SubstLc qualifier.
+Proof.
+  unfold SubstLc.
+  (* intros ϕ Hlc x u Hu. *)
+  destruct 1. intros Hu.
+  econstructor.
+  srewrite Vector.to_list_Forall.
+  rewrite Vector.to_list_map.
+  rewrite Forall_map.
+  eapply Forall_impl; eauto.
+  simpl. intros. fold_syntax_class. lc_solver1. fold_syntax_class. apply subst_lc; eauto.
+Qed.
+Arguments SubstLc_qualifier /.
+
+#[global] Instance FvOfSubstClosed_qualifier: FvOfSubstClosed qualifier.
+Proof.
+  unfold FvOfSubstClosed.
+  intros x u ϕ Hx.
+  destruct ϕ; ln_simpl. clear prop. induction vals; simpl; intros.
+  my_set_solver. fold_syntax_class.
+  rewrite fv_of_subst_closed; eauto.
+  setoid_rewrite IHvals; eauto. my_set_solver.
+Qed.
+Arguments FvOfSubstClosed_qualifier /.
+
+#[global] Instance OpenNotInEq_qualifier: OpenNotInEq qualifier.
+Proof.
+  unfold OpenNotInEq.
+  intros x ϕ k H.
+  destruct ϕ; ln_simpl.
+  f_equal.
+  clear - H.
+  induction vals; simpl; eauto.
+  f_equal. apply open_not_in_eq. my_set_solver.
+  auto_apply. my_set_solver.
+Qed.
+Arguments OpenNotInEq_qualifier /.
+
+#[global] Instance LcSubst_qualifier: LcSubst qualifier.
+Proof.
+  unfold LcSubst.
+  intros x u ϕ Hlc Hu.
+  sinvert Hlc.
+  destruct ϕ. ln_simpl. simplify_eq.
+  econstructor.
+  srewrite Vector.to_list_Forall.
+  srewrite Vector.to_list_map.
+  srewrite Forall_map.
+  eapply Forall_impl; eauto.
+  simpl. intros. fold_syntax_class. lc_solver1. fold_syntax_class. eapply lc_subst; eauto.
+Qed.
+
+#[global] Instance OpenRecLc_qualifier: OpenRecLc qualifier.
+Proof.
+  unfold OpenRecLc.
+  destruct 1. intros. ln_simpl.
+  f_equal.
+  rewrite <- Vector.map_id.
+  apply Vector.map_ext_in.
+  rewrite Vector.Forall_forall in H.
+  intros. fold_syntax_class. rewrite open_rec_lc; eauto.
+Qed.
+Arguments OpenRecLc_qualifier /.
+
+#[global] Instance OpenIdemp_qualifier: OpenIdemp qualifier.
+Proof.
+  unfold OpenIdemp.
+  destruct t; intros. ln_simpl.
+  f_equal.
+  rewrite Vector.map_map.
+  apply Vector.map_ext_in.
+  intros. do 2 fold_syntax_class. rewrite open_idemp; eauto.
+Qed.
+Arguments OpenIdemp_qualifier /.
+
+#[global] Instance OpenSwap_qualifier: OpenSwap qualifier.
+Proof.
+  unfold OpenSwap.
+  destruct t; intros. ln_simpl.
+  f_equal. rewrite !Vector.map_map.
+  apply Vector.map_ext.
+  intros. do 2 fold_syntax_class. rewrite open_swap; eauto.
+Qed.
+Arguments OpenSwap_qualifier /.
+
+#[global] Instance OpenLcRespect_qualifier: OpenLcRespect qualifier.
+Proof.
+  unfold OpenLcRespect.
+  intros ϕ u v k H. sinvert H.
+  destruct ϕ. ln_simpl. simplify_eq.
+  econstructor.
+  srewrite Vector.to_list_Forall.
+  srewrite Vector.to_list_map.
+  srewrite Forall_map.
+  eapply Forall_impl; eauto.
+  simpl. intros. fold_syntax_class. lc_solver1. fold_syntax_class. eapply open_lc_respect; eauto.
+Qed.
+Arguments OpenLcRespect_qualifier /.
+
+Arguments qualifier_and : simpl never.
+
+Class SubstBody2 A `{Stale aset A} `{open: Open value A} `{Subst value A} `{lc : Lc A}:= subst_body :
+forall x (u: value) (e: A), body2 e -> lc_value u -> body2 ({x := u} e).
+
+#[global] Instance SubstBody2_qualifier: SubstBody2 qualifier.
+Proof.
+  unfold SubstBody2.
+  unfold body2.
+  destruct 1. intros Hu.
+  auto_exists_L. intros y1 Hy1 y2 Hy2.
+  specialize_with y1.
+  specialize_with y2.
+  rewrite <- !subst_open_var by (eauto; my_set_solver).
+  pose subst_lc. eauto.
+Qed.
+Arguments SubstBody2_qualifier /.
+
+Class BodySubst A `{Stale aset A} `{Open value A} `{Subst value A} `{Lc A} := body_subst :
+forall (x: atom) (u: value) (e: A), body ({x := u} e) -> lc_value u -> body e.
+
+#[global] Instance BodySubst_qualifier: BodySubst qualifier.
+Proof.
+  unfold BodySubst.
+  unfold body.
+  destruct 1. intros Hu.
+  auto_exists_L. intros y Hy.
+  specialize_with y.
+  eapply lc_subst; eauto.
+  rewrite -> !subst_open_var; eauto. my_set_solver.
+Qed.
+Arguments BodySubst_qualifier /.
+
+Class Body2Subst A `{Stale aset A} `{Open value A} `{Subst value A} `{Lc A} := body2_subst:
+forall (x: atom) (u: value) (e: A), body2 ({x := u} e) -> lc_value u -> body2 e.
+
+#[global] Instance Body2Subst_qualifier: Body2Subst qualifier.
+Proof.
+  unfold Body2Subst.
+  unfold body2.
+  destruct 1. intros Hu.
+  auto_exists_L. intros y1 Hy1 y2 Hy2.
+  specialize_with y1. specialize_with y2.
+  eapply lc_subst; eauto.
+  rewrite -> !subst_open_var; eauto; my_set_solver.
+Qed.
+Arguments Body2Subst_qualifier /.
+
+Lemma lc_phi1_and ϕ1 ϕ2:
+  body ϕ1 -> body ϕ2 -> body (ϕ1 & ϕ2).
+Proof.
+  intros. unfold body in *. unfold Body_default in *. simp_hyps.
+  auto_exists_L. intros y1 Hy1.
+  specialize_with y1. specialize_with y1.
+  setoid_rewrite qualifier_and_open.
+  apply lc_qualifier_and; eauto.
+Qed.
+
+Lemma lc_phi2_and ϕ1 ϕ2:
+  body2 ϕ1 -> body2 ϕ2 -> body2 (ϕ1 & ϕ2).
+Proof.
+  intros. unfold body2 in *. unfold Body2_default in *. simp_hyps.
+  auto_exists_L. intros y1 Hy1 y2 Hy2.
+  specialize_with y1. specialize_with y2.
+  specialize_with y1. specialize_with y2.
+  setoid_rewrite qualifier_and_open. setoid_rewrite qualifier_and_open.
+  apply lc_qualifier_and; eauto.
+Qed.
+
+Lemma lc_phi1_body: ∀ n vals prop,
+    body (@qual n vals prop) -> Vector.Forall (fun v => body v) vals.
+Proof.
+  intros. subst. sinvert H.
+  rewrite Vector.Forall_forall. intros.
+  auto_exists_L. intros.
+  ospecialize * (H0 x0). my_set_solver.
+  sinvert H0.
+  apply Classical_Prop.EqdepTheory.inj_pair2 in H4.
+  apply Classical_Prop.EqdepTheory.inj_pair2 in H5.
+  subst.
+  rewrite VectorSpec.Forall_map in H3.
+  rewrite Vector.Forall_forall in H3. eauto.
+Qed.
+
+Lemma lc_phi2_body: ∀ n vals prop,
+    body2 (@qual n vals prop) ->
+    Vector.Forall (fun v => body2 v) vals.
+Proof.
+  unfold body2. unfold Body2_default. intros. subst. sinvert H.
+  rewrite Vector.Forall_forall. intros.
+  auto_exists_L. intros.
+  ospecialize * (H0 x0 _ y). my_set_solver. my_set_solver.
+  sinvert H0.
+  apply Classical_Prop.EqdepTheory.inj_pair2 in H5.
+  apply Classical_Prop.EqdepTheory.inj_pair2 in H6.
+  subst.
+  repeat rewrite VectorSpec.Forall_map in H4.
+  rewrite Vector.Forall_forall in H4. eauto.
+Qed.
+
+(* NOTE: Very very annoying, a reverse version of map_ext, using classical logic *)
+Lemma vector_map_ext_in' {A B: Type} (f g: A -> B) {n: nat} (vec: vec A n):
+  vmap f vec = vmap g vec -> (forall x, @Vector.In A x n vec -> f x = g x).
+Proof.
+  induction vec; simpl; intros.
+  - inversion H0.
+  - sinvert H.
+    apply Classical_Prop.EqdepTheory.inj_pair2 in H3.
+    sinvert H0; eauto.
+    apply Classical_Prop.EqdepTheory.inj_pair2 in H5. subst.
+    eapply IHvec in H3; eauto.
+Qed.
+
+#[global] Instance Fact1_qualifier: Fact1 qualifier.
+Proof.
+    unfold Fact1.
+    intros u v ϕ i j Hij Hijuv.
+  destruct ϕ. ln_simpl. f_equal.
+  rewrite <- Vector.map_id.
+  apply Vector.map_ext_in.
+  simplify_eq.
+  (* apply Classical_Prop.EqdepTheory.inj_pair2 in Hij. *)
+  rewrite Vector.map_map in Hijuv.
+  intros.
+  eapply vector_map_ext_in' in Hijuv; eauto.
+  do 2 fold_syntax_class.
+  eapply fact1; eauto.
+Qed.
+
+Class Fact1Twice A `{Stale aset A} `{Open value A} := fact1_twice :
+forall (u v1 v2: value) (e: A) i j1 j2,
+    i <> j1 -> i <> j2 -> j1 <> j2 ->
+    {i ~> u} ({j1 ~> v1} ({j2 ~> v2} e)) = {j1 ~> v1} ({j2 ~> v2} e) -> {i ~> u} e = e.
+
+#[global] Instance Fact1Twice_all 
+  (A : Type)
+  (staleA : Stale A)
+  (openA  : Open value A)
+  (fact1A : @Fact1 A staleA openA)
+  : @Fact1Twice A staleA openA.
+Proof.
+  unfold Fact1Twice.
+  intros u v1 v2 e i j1 j2 Hij1 Hij2 Hj1j2 Hij1v2v1.
+  assert ({i ~> u} ({j2 ~> v2} e) = {j2 ~> v2} e).
+  eapply fact1 with (j := j1) (v:= v1); eauto.
+  eapply fact1 with (j := j2) (v:= v2); eauto.
+Qed.
+Arguments Fact1Twice_all /.
+
+Class OpenRecBody A `{Stale aset A} `{Open value A} `{Lc A} := open_rec_body :
+forall (e: A), body e -> forall (k: nat) (v: value), {S k ~> v} e = e.
+
+#[global] Instance OpenRecBody_qualifier: OpenRecBody qualifier.
+Proof.
+  unfold OpenRecBody.
+  intros ϕ Hlc k v. destruct ϕ. apply lc_phi1_body in Hlc.
+  ln_simpl. f_equal.
+  rewrite <- Vector.map_id.
+  apply Vector.map_ext_in.
+  intros.
+  rewrite Vector.Forall_forall in Hlc.
+  ospecialize * Hlc; eauto.
+  destruct Hlc.
+  auto_pose_fv y.
+  apply fact1 with (j := 0) (v:= y). lia.
+  rewrite open_rec_lc; eauto. auto_apply. my_set_solver.
+Qed.
+Arguments OpenRecBody_qualifier /.
+
+Class OpenRecBody2 A `{Stale aset A} `{Open value A} `{Lc A} := open_rec_body2 :
+forall (e: A), body2 e -> forall (k: nat) (v: value), {S (S k) ~> v} e = e.
+
+(* NOTE: Very very annoying, when qualifier has builtin 1 or 2 arguments. *)
+
+#[global] Instance OpenRecBody2_qualifier: OpenRecBody2 qualifier.
+Proof.
+  unfold OpenRecBody2.
+  intros ϕ Hlc k v. destruct ϕ. apply lc_phi2_body in Hlc.
+  ln_simpl. f_equal.
+  rewrite <- Vector.map_id.
+  apply Vector.map_ext_in.
+  intros.
+  rewrite Vector.Forall_forall in Hlc.
+  ospecialize * Hlc; eauto.
+  destruct Hlc.
+  auto_pose_fv y1. auto_pose_fv y2.
+  ospecialize * (H0 y1 _ y2); eauto. my_set_solver. my_set_solver.
+  fold_syntax_class.
+  eapply (fact1_twice _ y1 y2 _ _ 0 1); eauto.
+  rewrite open_rec_lc; eauto.
+Qed.
+Arguments OpenRecBody2_qualifier /.
